Kill a few assumptions in Copy.Vec, guarantee that vector copies are 16 bytes

src/lib/data/Kuiper.Array.Vectorized.fsti
@@ -11,23 +11,25 @@ module SZ = Kuiper.SizeT
 
 inline_for_extraction noextract
 unfold
-class has_vec_cpy (et : Type) = {
+class has_vec_cpy (et : Type) {| sized et |} = {
   [@@@FStar.Tactics.Typeclasses.no_method] _chunk : szp;
+  [@@@FStar.Tactics.Typeclasses.no_method] _pf : squash (_chunk * size #et == 16);
+  (* ^ Vectorized copies are always 16 bytes wide. *)
 }
 
 unfold
 inline_for_extraction noextract
-let chunk (et : Type) {| hvc : has_vec_cpy et |} : szp =
+let chunk (et : Type) {| sized et, hvc : has_vec_cpy et |} : szp =
   match hvc with
-  | Mkhas_vec_cpy chunk -> chunk
+  | Mkhas_vec_cpy chunk _ -> chunk
 
 unfold
 inline_for_extraction noextract
-instance has_vec_cpy_float : has_vec_cpy float = { _chunk = 4sz; }
+instance has_vec_cpy_float : has_vec_cpy float = { _chunk = 4sz; _pf = ez; }
 
 unfold
 inline_for_extraction noextract
-instance has_vec_cpy_half  : has_vec_cpy half  = { _chunk = 8sz; }
+instance has_vec_cpy_half  : has_vec_cpy half  = { _chunk = 8sz; _pf = ez; }
 
 (* These three operations are essentially the same. We need different
    variants since gpu_array is a different type from array. Sadly the
