src/lib/poly/gemm/Kuiper.Poly.GEMM.BlockTiling2D.fst
@@ -102,7 +102,7 @@ let kpost1
   own_thread_tile gC bm bn tm tn bid tid
 
 let barrier_p
-  (#et : Type0) {| has_vec_cpy et |}
+  (#et : Type0) {| sized et, has_vec_cpy et |}
   (#bm #bn #bk : szp)
   (#l1 : mlayout bm bk)
   (#l2 : mlayout bk bn)
@@ -119,7 +119,7 @@ let barrier_p
       live_tile_stride_cells m2 nthr tid
 
 let barrier_q
-  (#et : Type0) {| has_vec_cpy et |}
+  (#et : Type0) {| sized et, has_vec_cpy et |}
   (#bm #bn #bk : szp)
   (#l1 : mlayout bm bk)
   (#l2 : mlayout bk bn)
@@ -130,7 +130,7 @@ let barrier_q
   fun it tid -> barrier_p m1 m2 nthr (it+1) tid (* flip flop *)
 
 let barrier_tok
-  (#et : Type0) {| has_vec_cpy et |}
+  (#et : Type0) {| sized et, has_vec_cpy et |}
   (#bm #bn #bk : szp)
   (* This is defined over the base shared gpu_arrays, as
   this spec must make sense before the arrays are viewed as
@@ -150,7 +150,7 @@ let barrier_tok
 
 unfold
 let kpre
-  (#et : Type0) {| scalar et, has_vec_cpy et |}
+  (#et : Type0) {| scalar et, v : has_vec_cpy et |}
   (comb : binop et)
   (#rows #shared #cols : szp)
   (#lA : mlayout rows shared)
@@ -178,11 +178,11 @@ let kpre
   kpre1 comb gA eA gB eB gC bm bn bk tm tn fA fB bid tid **
   (exists* (x : seq _). fst sh |-> Frac (1.0R /. (bm/tm * (bn/tn))) x) **
   (exists* (x : seq _). fst (snd sh) |-> Frac (1.0R /. (bm/tm * (bn/tn))) x) **
-  barrier_tok slA slB (fst sh) (fst (snd sh)) 0 (bm/tm * (bn/tn)) tid
+  barrier_tok #_ #_ #v slA slB (fst sh) (fst (snd sh)) 0 (bm/tm * (bn/tn)) tid
 
 unfold
 let kpost
-  (#et : Type0) {| scalar et, has_vec_cpy et |}
+  (#et : Type0) {| scalar et, v : has_vec_cpy et |}
   (comb : binop et)
   (#rows #shared #cols : szp)
   (#lA : mlayout rows shared)
@@ -210,7 +210,7 @@ let kpost
   kpost1 comb gA eA gB eB gC bm bn bk tm tn fA fB bid tid **
   (exists* (x : seq _). fst sh |-> Frac (1.0R /. (bm/tm * (bn/tn))) x) **
   (exists* (x : seq _). fst (snd sh) |-> Frac (1.0R /. (bm/tm * (bn/tn))) x) **
-  barrier_tok slA slB (fst sh) (fst (snd sh)) (2 * (shared/bk)) (bm/tm * (bn/tn)) tid
+  barrier_tok #_ #_ #v slA slB (fst sh) (fst (snd sh)) (2 * (shared/bk)) (bm/tm * (bn/tn)) tid
 
 inline_for_extraction noextract
 fn subproducts2d
